Fix heap sort specification.

code/Yazi.Tree.fst
@@ -42,39 +42,44 @@ let smaller
   else
     false
 
-#set-options "--z3refresh --z3rlimit 32768 --fuel 0 --ifuel 0"
 inline_for_extraction
 let smallest
   (heap: tree_heap_t) (hl: heap_len_t)
   (tl: tree_len_t) (tree: B.lbuffer ct_data tl)
   (depth: tree_depth_t) (i: U32.t{U32.v i < tl})
   (root: Ghost.erased (heap_internal_index_t hl))
-  (j: heap_internal_index_t hl):
+  (hole: heap_internal_index_t hl):
   ST.Stack U32.t
   (requires fun h ->
     let open U32 in
-    v root <= v j /\
+    let partial_well_formed = SH.partial_well_formed h heap hl tl tree depth in
+    v root <= v hole /\
     htd_seperate h heap tree depth /\
-    SH.element_in_range h heap hl tl /\
-    SH.smaller h tl tree depth (B.as_seq h heap).[v j] i /\
-    SH.partial_well_formed h heap hl tl tree depth root)
+    SH.smaller h tl tree depth (B.as_seq h heap).[v hole] i /\
+    (v root == v hole ==>
+      partial_well_formed (root +^ 1ul) /\
+      (B.as_seq h heap).[v root] == i) /\
+    (v root < v hole ==> partial_well_formed root))
   (ensures fun h0 res h1 ->
     let heap = B.as_seq h1 heap in let hl = U32.v hl in
-    let j = U32.v j in let res = U32.v res in
+    let root = U32.v root in let hole = U32.v hole in
+    let res = U32.v res in
     let smaller' = SH.smaller h1 tl tree depth in
     
     B.modifies B.loc_none h0 h1 /\
-    res <= hl /\ (res == 0 \/ res == j * 2 \/ res == j * 2 + 1) /\
+    res <= hl /\ (res == 0 \/ res == hole * 2 \/ res == hole * 2 + 1) /\
     (let k = if res = 0 then i else heap.[res] in
     k `smaller'` i /\
-    k `smaller'` heap.[j * 2] /\
-    (j * 2 + 1 <= hl ==> k `smaller'` heap.[j * 2 + 1]) /\
-    heap.[j] `smaller'` k)) =
+    k `smaller'` heap.[hole * 2] /\
+    (hole * 2 + 1 <= hl ==> k `smaller'` heap.[hole * 2 + 1]) /\
+    (root == hole ==> k `smaller'` heap.[hole]) /\
+    (root < hole ==> heap.[hole] `smaller'` k))) =
   let open U32 in
-  let l = j *^ 2ul in
+  let l = hole *^ 2ul in
   let r = l +^ 1ul in
   let le = heap.(l) in
   let smaller' = smaller tl tree depth in
+  let h = ST.get () in
   if r >^ hl then
     if i `smaller'` le then 0ul else l
   else
@@ -84,42 +89,55 @@ let smallest
     else
       if le `smaller'` re then l else r
 
-#set-options "--z3refresh --z3rlimit 32768 --fuel 0 --ifuel 0"
-[@CInline]
+#set-options "--z3refresh --z3rlimit 4096 --fuel 0 --ifuel 0"
+inline_for_extraction
 let rec do_pqdownheap
   (h_init: Ghost.erased HS.mem)
   (heap: tree_heap_t) (hl: heap_len_t)
   (tl: tree_len_t) (tree: B.lbuffer ct_data tl)
   (depth: tree_depth_t)
   (i: U32.t{U32.v i < tl})
-  (k: Ghost.erased (heap_internal_index_t hl))
-  (j: heap_index_t hl):
+  (root: Ghost.erased (heap_internal_index_t hl))
+  (hole: heap_index_t hl):
   ST.Stack unit
   (requires fun h ->
     let open U32 in
-    v k <= v j /\
-    (B.as_seq h_init heap).[v k] == i /\
+    v root <= v hole /\
+    (B.as_seq h_init heap).[v root] == i /\
     htd_seperate h heap tree depth /\
-    SH.smaller h tl tree depth (B.as_seq h heap).[U32.v j] i /\
-    SH.partial_well_formed h heap hl tl tree depth k /\
-    SH.permutation_partial (B.as_seq h_init heap) (B.as_seq h heap) k j)
+    SH.smaller h tl tree depth (B.as_seq h heap).[v hole] i /\
+    (v root == v hole ==> SH.partial_well_formed h heap hl tl tree depth (root +^ 1ul)) /\
+    (v root < v hole ==> SH.partial_well_formed h heap hl tl tree depth root) /\
+    SH.permutation_partial (B.as_seq h_init heap) (B.as_seq h heap) root hole)
   (ensures fun h0 _ h1 ->
     B.modifies (B.loc_buffer heap) h0 h1 /\
-    SH.partial_well_formed h1 heap hl tl tree depth k)
-  (decreases U32.v hl / 2 - U32.v j) =
+    SH.partial_well_formed h1 heap hl tl tree depth root /\
+    Seq.permutation U32.t (B.as_seq h_init heap) (B.as_seq h1 heap))
+  (decreases U32.v hl / 2 - U32.v hole) =
   let open U32 in
-  let internal = hl /^ 2ul in
-  if j >^ internal then
-    heap.(j) <- i
+  if hole >^ hl /^ 2ul then 
+    heap.(hole) <- i
   else
-    let s = smallest heap hl tl tree depth i k j in
+    let s = smallest heap hl tl tree depth i root hole in
     if s = 0ul then
-      heap.(j) <- i
+      heap.(hole) <- i
     else begin
-      let h0 = ST.get () in
-      let s' = heap.(s) in
-      heap.(j) <- s';
-      let h1 = ST.get () in
-      upd_count (B.as_seq h0 heap) (B.as_seq h1 heap) (v j) s';
-      do_pqdownheap h_init heap hl tl tree depth i k s
+      heap.(hole) <- heap.(s);
+      do_pqdownheap h_init heap hl tl tree depth i root s
     end
+
+inline_for_extraction
+let pqdownheap
+  (heap: tree_heap_t) (hl: heap_len_t)
+  (tl: tree_len_t) (tree: B.lbuffer ct_data tl)
+  (depth: tree_depth_t)
+  (i: heap_internal_index_t hl):
+  ST.Stack unit
+  (requires fun h ->
+    htd_seperate h heap tree depth /\
+    SH.partial_well_formed h heap hl tl tree depth (U32.add i 1ul))
+  (ensures fun h0 _ h1 ->
+    B.modifies (B.loc_buffer heap) h0 h1 /\
+    SH.partial_well_formed h1 heap hl tl tree depth i /\
+    Seq.permutation U32.t (B.as_seq h0 heap) (B.as_seq h1 heap)) =
+  do_pqdownheap (ST.get ()) heap hl tl tree depth heap.(i) i i
